src/ShouldBuild.v
@@ -35,8 +35,7 @@ From Perennial.program_proof.lockservice Require
      bank_proof incr_proof incr_proxy_proof two_pc_example. *)
 
 From Perennial.goose_lang Require
-     ffi.append_log_ffi
-     ffi.kvs_ffi.
+     ffi.append_log_ffi.
 From Perennial.tutorial Require
      ipm_extensions.
 
